cp

vale/code/arch/x64/interop/Vale.AsLowStar.Wrapper.fst
@@ -143,19 +143,18 @@ let mem_correspondence_refl (args:list arg)
 ////////////////////////////////////////////////////////////////////////////////
 
 let prediction_rel
-          (code:V.va_code)
-          (args:IX64.arity_ok arg)
           (num_stack_slots:nat)
-          (pre:VSig.vale_pre_tl [])
           (post:VSig.vale_post_tl [])
-          (v:VSig.vale_sig_tl args (coerce code) pre post)
-          (h0:mem_roots args{LSig.(to_low_pre pre args num_stack_slots h0)})
-          (s0:TS.traceState)
-          (push_h0:mem_roots args)
-          (alloc_push_h0:mem_roots args)
-          (sb:IX64.stack_buffer{mem_roots_p alloc_push_h0 (IX64.arg_of_b8 sb::args)})
-          (fuel_mem:(nat & ME.mem))
-          (s1:TS.traceState) : prop =
+   : IX64.prediction_rel_t
+   = fun (code:V.va_code)
+       (args:IX64.arity_ok arg)
+       (h0:mem_roots args)
+       (s0:TS.traceState)
+       (push_h0:mem_roots args)
+       (alloc_push_h0:mem_roots args)
+       (sb:IX64.stack_buffer{mem_roots_p alloc_push_h0 (IX64.arg_of_b8 sb::args)})
+       (fuel_mem:(nat & ME.mem))
+       (s1:TS.traceState) ->
     let open Interop.Adapters in
     let h1_pre_pop = hs_of_mem (snd fuel_mem) in
     HS.poppable h1_pre_pop /\ (
@@ -176,7 +175,7 @@ let vale_lemma_as_prediction
           (post:VSig.vale_post_tl [])
           (v:VSig.vale_sig_tl args (coerce code) pre post)
           (h0:mem_roots args{LSig.(to_low_pre pre args num_stack_slots h0)})
-   : IX64.prediction (coerce code) args h0 (prediction_rel code args num_stack_slots pre post v h0)
+   : IX64.prediction (prediction_rel num_stack_slots post) (coerce code) args h0
    = fun s0 push_h0 alloc_push_h0 sb ->
        let va_s0 = create_initial_vale_state args alloc_push_h0 sb in
        core_create_lemma args alloc_push_h0 sb;
@@ -282,7 +281,7 @@ let rec wrap (#dom:list td)
            let h0 = ST.get () in
            let prediction =
              vale_lemma_as_prediction _ _ num_stack_slots _ _ v h0 in
-           let _ = IX64.wrap (coerce code) args h0 prediction in
+           let _ = IX64.wrap_variadic (coerce code) args h0 prediction in
            ()
       in
       f <: lowstar_typ #[] code args num_stack_slots pre post
@@ -290,8 +289,67 @@ let rec wrap (#dom:list td)
       fun (x:td_as_type hd) ->
         wrap
           code
-          ((| hd, x |) :: args)
+          IX64.(x ++ args)
           num_stack_slots
           (elim_1 pre x)
           (elim_1 post x)
           (VSig.elim_vale_sig_cons hd tl args pre post v x)
+
+////////////////////////////////////////////////////////////////////////////////
+//Wrap abstract
+////////////////////////////////////////////////////////////////////////////////
+
+let rec prediction_builder_t
+       (code:V.va_code)
+       (dom:list td)
+       (args:list arg{List.length dom + List.length args < IX64.max_arity})
+       (num_stack_slots:nat)
+       (pre:VSig.vale_pre_tl dom)
+       (post:VSig.vale_post_tl dom)
+   = let open IX64 in
+     match dom with
+     | [] ->
+       h0:HS.mem{mem_roots_p h0 args /\
+                 LSig.to_low_pre pre args num_stack_slots h0} ->
+       prediction_t (coerce code) dom args (prediction_rel num_stack_slots post) h0
+
+     | hd::tl ->
+       x:td_as_type hd ->
+       prediction_builder_t code tl (x ++ args) num_stack_slots (elim_1 pre x) (elim_1 post x)
+
+let rec mk_prediction
+       (code:V.va_code)
+       (dom:list td)
+       (args:list arg{List.length dom + List.length args < IX64.max_arity})
+       (num_stack_slots:nat)
+       (pre:VSig.vale_pre_tl dom)
+       (post:VSig.vale_post_tl dom)
+       (v:VSig.vale_sig_tl args (coerce code) pre post)
+    : prediction_builder_t code dom args num_stack_slots pre post
+    = let open IX64 in
+      match dom with
+      | [] ->
+        vale_lemma_as_prediction _ _ num_stack_slots _ _ v
+      | hd::tl ->
+        fun (x:td_as_type hd) ->
+        mk_prediction
+          code
+          tl
+          (x ++ args)
+          num_stack_slots
+          (elim_1 pre x)
+          (elim_1 post x)
+          (VSig.elim_vale_sig_cons hd tl args pre post v x)
+
+////////////////////////////////////////////////////////////////////////////////
+//test
+////////////////////////////////////////////////////////////////////////////////
+let _t = TD_Buffer ME.TUInt64
+unfold
+let _dom = [_t; _t]
+assume val _pre : VSig.vale_pre _dom
+assume val _post : VSig.vale_post _dom
+assume val _n : nat
+assume val _v: VSig.vale_sig _pre _post
+assume val _c: V.va_code
+open Interop.X64
